thys/Untyped_Lambda_Calculus/LC_Beta.thy
@@ -1,0 +1,207 @@
+theory LC_Beta 
+imports LC  "../../Curry_LFP" "../Generic_Barendregt_Enhanced_Rule_Induction"
+begin
+
+(* INSTANTIATING THE ABSTRACT SETTING: *)
+
+(* INSTATIATING THE Small LOCALE (INDEPENDENTLY OF THE CONSIDERED INDUCTIVE PREDICATE *) 
+
+print_locales
+interpretation Small where dummy = "undefined :: var" 
+apply standard
+  apply (simp add: infinite_var)  
+  using term_prevar_term_prevar_sumterm_prevar_prodIDterm_prevar_prodID_class.regular by blast
+ 
+
+(* AN EXAMPLE INDUCTIVE DEFINITION *)
+(* (a reduced form of) small step semantics *) 
+
+inductive step :: "trm \<Rightarrow> trm \<Rightarrow> bool" where
+  Beta: "step (App (Abs x e1) e2) (tvsubst (VVr(x:=e2)) e1)"
+| AppL: "step e1 e1' \<Longrightarrow> step (App e1 e2) (App e1' e2)"
+| Xi: "step e e' \<Longrightarrow> step (Abs x e) (Abs x e')"
+|PBeta: "step e1 e1' \<Longrightarrow> step e2 e2' \<Longrightarrow> step (App (Abs x e1) e2) (tvsubst (VVr(x:=e2')) e1')"
+
+thm step_def
+
+(* INSTANTIATING THE Components LOCALE: *)
+
+type_synonym T = "trm \<times> trm"
+type_synonym V = "var list" (* in this case, could have also taken to be 'a option; 
+and the most uniform approach would have been 'a + unit + 'a + 'a *)
+
+
+definition Tmap :: "(var \<Rightarrow> var) \<Rightarrow> T \<Rightarrow> T" where 
+"Tmap f \<equiv> map_prod (rrename_term f) (rrename_term f)"
+
+fun Tfvars :: "T \<Rightarrow> var set" where 
+"Tfvars (e1,e2) = FFVars_term e1 \<union> FFVars_term e2"
+
+definition Vmap :: "(var \<Rightarrow> var) \<Rightarrow> V \<Rightarrow> V" where 
+"Vmap \<equiv> map"
+
+fun Vfvars :: "V \<Rightarrow> var set" where 
+"Vfvars v = set v"
+
+interpretation Components where dummy = "undefined :: var" and 
+Tmap = Tmap and Tfvars = Tfvars
+and Vmap = Vmap and Vfvars = Vfvars 
+apply standard unfolding ssbij_def Tmap_def Vmap_def
+  using small_Un small_def term.card_of_FFVars_bounds
+  apply (auto simp: term.rrename_id0s map_prod.comp term.rrename_comp0s inf_A)  
+  by auto 
+
+definition G :: "(T \<Rightarrow> bool) \<Rightarrow> V \<Rightarrow> T \<Rightarrow> bool"
+where
+"G \<equiv> \<lambda>R v t.  
+         (\<exists>x e1 e2. v = [x] \<and> fst t = App (Abs x e1) e2 \<and> snd t = tvsubst (VVr(x := e2)) e1)
+         \<or>
+         (\<exists>e1 e1' e2. v = [] \<and> fst t = App e1 e2 \<and> snd t = App e1' e2 \<and> R (e1,e1')) 
+         \<or>
+         (\<exists>x e e'. v = [x] \<and> fst t = Abs x e \<and> snd t = Abs x e' \<and> R (e,e'))
+         \<or>
+         (\<exists>x e1 e1' e2 e2'. v = [x] \<and> fst t = App (Abs x e1) e2 \<and> snd t = tvsubst (VVr(x := e2')) e1' \<and> 
+            R (e1,e1') \<and> R (e2,e2'))"
+
+
+(* VERIFYING THE HYPOTHESES FOR BARENDREGT-ENHANCED INDUCTION: *)
+
+lemma GG_mono: "R \<le> R' \<Longrightarrow> G R v t \<Longrightarrow> G R' v t"
+unfolding G_def by fastforce
+
+lemma GG_equiv: "ssbij \<sigma> \<Longrightarrow> G R v t \<Longrightarrow> G (\<lambda>t'. R (Tmap (inv \<sigma>) t')) (Vmap \<sigma> v) (Tmap \<sigma> t)"
+unfolding G_def apply(elim disjE)
+  subgoal apply(rule disjI1)
+  subgoal apply(elim exE) subgoal for x e1 e2 
+  apply(rule exI[of _ "\<sigma> x"])
+  apply(rule exI[of _ "rrename_term \<sigma> e1"]) apply(rule exI[of _ "rrename_term \<sigma> e2"])
+  apply(cases t) unfolding ssbij_def small_def Tmap_def Vmap_def apply simp
+  apply(subst rrename_tvsubst_comp) by auto  . .
+  (* *)
+  subgoal apply(rule disjI2, rule disjI1)
+  subgoal apply(elim exE) subgoal for e1 e1' e2
+  apply(rule exI[of _ "rrename_term \<sigma> e1"]) apply(rule exI[of _ "rrename_term \<sigma> e1'"]) 
+  apply(rule exI[of _ "rrename_term \<sigma> e2"])
+  apply(cases t) unfolding ssbij_def small_def Tmap_def Vmap_def 
+  by (simp add: term.rrename_comps) . . 
+  (* *)
+  subgoal apply(rule disjI2, rule disjI2, rule disjI1)
+  subgoal apply(elim exE) subgoal for x e e'
+  apply(rule exI[of _ "\<sigma> x"])
+  apply(rule exI[of _ "rrename_term \<sigma> e"]) apply(rule exI[of _ "rrename_term \<sigma> e'"]) 
+  apply(cases t) unfolding ssbij_def small_def Tmap_def Vmap_def 
+  by (simp add: term.rrename_comps) . . 
+  (* *)
+  subgoal apply(rule disjI2, rule disjI2, rule disjI2)
+  subgoal apply(elim exE) subgoal for x e1 e1' e2 e2'
+  apply(rule exI[of _ "\<sigma> x"])
+  apply(rule exI[of _ "rrename_term \<sigma> e1"]) apply(rule exI[of _ "rrename_term \<sigma> e1'"]) 
+  apply(rule exI[of _ "rrename_term \<sigma> e2"]) apply(rule exI[of _ "rrename_term \<sigma> e2'"]) 
+  apply(cases t) unfolding ssbij_def small_def Tmap_def Vmap_def 
+  apply (simp add: term.rrename_comps) apply(subst rrename_tvsubst_comp) by auto
+ . . . 
+  
+
+lemma fresh: "\<exists>xx. xx \<notin> Tfvars t"  
+by (metis Abs_avoid Tfvars.elims term.card_of_FFVars_bounds term.set(2))
+
+lemma GG_fresh: 
+"(\<forall>\<sigma> t. ssbij \<sigma> \<and> R t \<longrightarrow> R (Tmap \<sigma> t)) \<Longrightarrow> G R v t \<Longrightarrow> 
+ \<exists>w. Vfvars w  \<inter> Tfvars t = {} \<and> G R w t"
+using fresh[of t] unfolding G_def Tmap_def Vmap_def apply safe
+  subgoal for xx x e1 e2
+  apply(rule exI[of _ "[xx]"])  
+  apply(rule conjI)
+    subgoal unfolding ssbij_def small_def Vmap_def by auto 
+    subgoal apply(rule disjI1) 
+    apply(rule exI[of _ "xx"]) 
+    apply(rule exI[of _ "rrename_term (id(x:=xx,xx:=x)) e1"])
+    apply(rule exI[of _ "e2"])
+    apply(cases t)  apply simp apply(intro conjI)
+      subgoal apply(subst Abs_rrename[of "id(x:=xx,xx:=x)"]) by auto
+      subgoal using tvsubst_Var_rrename_term by auto . .
+  (* *)
+  subgoal for xx e1 e1' e2
+  apply(rule exI[of _ "[]"])  
+  apply(rule conjI)
+    subgoal unfolding ssbij_def small_def Vmap_def by auto 
+    subgoal apply(rule disjI2, rule disjI1) 
+    apply(rule exI[of _ "e1"]) 
+    apply(rule exI[of _ "e1'"])
+    apply(rule exI[of _ "e2"]) 
+    apply(cases t)  apply simp . .
+  (* *)
+  subgoal for xx x e e'
+  apply(rule exI[of _ "[xx]"])  
+  apply(rule conjI)
+    subgoal unfolding ssbij_def small_def Vmap_def by auto 
+    subgoal apply(rule disjI2, rule disjI2, rule disjI1) 
+    apply(rule exI[of _ "xx"]) 
+    apply(rule exI[of _ "rrename_term (id(x:=xx,xx:=x)) e"])
+    apply(rule exI[of _ "rrename_term (id(x:=xx,xx:=x)) e'"])
+    apply(cases t)  apply simp apply(intro conjI)
+      subgoal apply(subst Abs_rrename[of "id(x:=xx,xx:=x)"]) by auto
+      subgoal apply(subst Abs_rrename[of "id(x:=xx,xx:=x)"]) by auto
+      subgoal by (metis supp_swap_bound Prelim.bij_swap ssbij_def) . . 
+  (* *)
+  subgoal for xx x e1 e1' e2 e2'
+  apply(rule exI[of _ "[xx]"])  
+  apply(rule conjI)
+    subgoal unfolding ssbij_def small_def Vmap_def by auto 
+    subgoal apply(rule disjI2, rule disjI2, rule disjI2)
+    apply(rule exI[of _ "xx"]) 
+    apply(rule exI[of _ "rrename_term (id(x:=xx,xx:=x)) e1"])
+    apply(rule exI[of _ "rrename_term (id(x:=xx,xx:=x)) e1'"])
+    apply(rule exI[of _ "e2"])
+    apply(rule exI[of _ "e2'"])
+    apply(cases t)  apply simp apply(intro conjI)
+      subgoal apply(subst Abs_rrename[of "id(x:=xx,xx:=x)"]) by auto
+      subgoal apply(subst tvsubst_Var_rrename_term) 
+      by (auto simp: FFVars_tvsubst split: if_splits)  
+      subgoal by (metis supp_swap_bound Prelim.bij_swap ssbij_def) . . . 
+  (* *)
+
+
+(* FINALLY, INTERPRETING THE Induct LOCALE: *)
+
+interpretation Induct where dummy = "undefined :: var" and 
+Tmap = Tmap and Tfvars = Tfvars
+and Vmap = Vmap and Vfvars = Vfvars and G = G
+apply standard 
+  using GG_mono GG_equiv GG_fresh by auto
+
+(* *)
+lemmas I_def = nitpick_unfold(178) 
+
+lemma step_I: "step t1 t2 = I (t1,t2)" 
+  unfolding step_def I_def lfp_curry2 apply(rule arg_cong2[of _ _ _ _ lfp], simp_all)
+  unfolding fun_eq_iff G_def apply safe
+    subgoal apply simp by metis
+    subgoal by auto
+    subgoal by auto
+    subgoal apply simp by metis
+    subgoal by auto
+    subgoal by auto
+    subgoal apply simp by metis
+    subgoal by auto .
+
+(* FROM ABSTRACT BACK TO CONCRETE: *)
+thm step.induct[no_vars]
+
+corollary BE_induct_step: "(\<And>p. small (Pfvars p)) \<Longrightarrow> 
+step t1 t2 \<Longrightarrow> 
+(\<And>x e e2 p. x \<notin> Pfvars p \<Longrightarrow> x \<notin> FFVars_term e2 \<Longrightarrow> R p (App (Abs x e) e2) (tvsubst (VVr(x := e2)) e)) \<Longrightarrow>
+(\<And>e1 e1' e2 p. step e1 e1' \<Longrightarrow> (\<forall>p'. R p' e1 e1') \<Longrightarrow> R p (App e1 e2) (App e1' e2)) \<Longrightarrow> 
+(\<And>e e' x p. x \<notin> Pfvars p \<Longrightarrow> step e e' \<Longrightarrow> (\<forall>p'. R p' e e') \<Longrightarrow> R p (Abs x e) (Abs x e')) \<Longrightarrow> 
+(\<And>x e e' e2 e2' p. x \<notin> Pfvars p \<Longrightarrow> step e e' \<Longrightarrow> (\<forall>p'. R p' e e') \<Longrightarrow> step e2 e2' \<Longrightarrow> (\<forall>p'. R p' e2 e2') \<Longrightarrow> 
+   x \<notin> FFVars_term e2 \<Longrightarrow> (x \<in> FFVars_term e' \<Longrightarrow> x \<notin> FFVars_term e2') \<Longrightarrow> 
+   R p (App (Abs x e) e2) (tvsubst (VVr(x := e2')) e')) \<Longrightarrow>
+ R p t1 t2"
+unfolding step_I
+apply(subgoal_tac "case (t1,t2) of (t1, t2) \<Rightarrow> R p t1 t2")
+  subgoal by auto
+  subgoal apply(erule BE_induct[where R = "\<lambda>p (t1,t2). R p t1 t2"])
+  unfolding G_def apply auto apply(subst (asm) FFVars_tvsubst) by (auto split: if_splits) .
+
+
+end
